src/tls/StreamDeltas.fst
@@ -29,7 +29,7 @@ let project_one_frag #i = function
       let d : DS.pre_fragment i = d in //A widening coercion as a proof hint, unpacking (d:fragment i (frange i)) to a pre_fr
       singleton (DataStream.Data d)
     | C.CT_Alert _ ad -> singleton (DataStream.Alert ad)
-    | _ -> Seq.createEmpty                 // other fragments are internal to TLS
+    | _ -> Seq.empty                 // other fragments are internal to TLS
 
 val project_deltas: #i:id -> fs:S.frags i -> GTot (deltas i)
 let project_deltas #i fs = MS.collect project_one_frag fs
